Weidenbach_Book/IsaSAT/IsaSAT_Initialisation_LLVM.thy
@@ -873,8 +873,6 @@ sepref_def empty_heuristics_stats_impl
   apply (rewrite in \<open>replicate _ False\<close> array_fold_custom_replicate)
   apply (rewrite at \<open>replicate _ False\<close> annotate_assn[where A=phase_saver_assn])
   apply (rewrite in \<open>replicate _ False\<close> larray_fold_custom_replicate)
-  apply (rewrite at \<open>(_, \<hole>, _,_,_,_)\<close> snat_const_fold[where 'a=64])
-  apply (rewrite at \<open>(_, _,_,\<hole>, _,_,_)\<close> snat_const_fold[where 'a=64])
   by sepref
 
 lemma finalise_init_code_alt_def:
