Weidenbach_Book/IsaSAT/IsaSAT_Rephase_State.thy
@@ -44,14 +44,14 @@ lemma rephase_heur_st_spec:
   apply (simp_all add:  twl_st_heur_def all_atms_st_def)
   done
 
-definition save_rephase_heur_stats :: \<open>nat \<Rightarrow> restart_heuristics \<Rightarrow> restart_heuristics nres\<close> where
+definition save_rephase_heur_stats :: \<open>64 word \<Rightarrow> restart_heuristics \<Rightarrow> restart_heuristics nres\<close> where
   \<open>save_rephase_heur_stats = (\<lambda>n (fast_ema, slow_ema, restart_info, wasted, \<phi>, relu).
     do {
       \<phi> \<leftarrow> phase_save_phase n \<phi>;
       RETURN (fast_ema, slow_ema, restart_info, wasted, \<phi>, relu)
   })\<close>
 
-definition save_rephase_heur :: \<open>nat \<Rightarrow> isasat_restart_heuristics \<Rightarrow> isasat_restart_heuristics nres\<close> where
+definition save_rephase_heur :: \<open>64 word \<Rightarrow> isasat_restart_heuristics \<Rightarrow> isasat_restart_heuristics nres\<close> where
   \<open>save_rephase_heur = (\<lambda>n heur.
   do {
   \<phi> \<leftarrow> save_rephase_heur_stats n (get_content heur);
@@ -68,12 +68,11 @@ lemma save_phase_heur_spec:
 
 definition save_phase_st :: \<open>isasat \<Rightarrow> isasat nres\<close> where
   \<open>save_phase_st = (\<lambda>S. do {
-      let M' = get_trail_wl_heur S;
+      let stats = get_stats_heur S;
+      let n = no_conflict_until stats;
       let heur = get_heur S;
-      ASSERT(isa_length_trail_pre M');
-      let n = isa_length_trail M';
       heur \<leftarrow> save_rephase_heur n heur;
-      RETURN (set_trail_wl_heur M' (set_heur_wl_heur heur S))
+      RETURN (set_heur_wl_heur heur S)
    })\<close>
 
 lemma save_phase_st_spec:
@@ -82,8 +81,6 @@ lemma save_phase_st_spec:
   apply (cases S')
   apply (refine_vcg save_phase_heur_spec[THEN order_trans, of \<open>all_atms_st S'\<close>])
   apply (simp_all add:  twl_st_heur_def isa_length_trail_pre all_atms_st_def flip: all_lits_st_alt_def)
-  apply (rule isa_length_trail_pre)
-  apply blast
   done
 
 end
